Proofs through qtesla_sign_compute_c_z except test_correctness
test_correctness still has assumptions related to left shifting that
Santiago is helping with the proofs on.

Push some assumptions about the output of polynomial math into the
functions themselves to remove assumptions from callers in the main file.

qtesla/code/Hacl.Impl.QTesla.Heuristic.Poly.fst
@@ -394,7 +394,7 @@ val poly_sub_correct:
   -> y: poly
   -> Stack unit
     (requires fun h -> live h result /\ live h x /\ live h y)
-    (ensures fun h0 _ h1 -> modifies1 result h0 h1)
+    (ensures fun h0 _ h1 -> modifies1 result h0 h1 /\ is_poly_montgomery h1 result)
 
 let poly_sub_correct result x y =
     push_frame();
@@ -412,7 +412,9 @@ let poly_sub_correct result x y =
         assume(is_elem temp);
         result.(i) <- temp
     );
-    pop_frame()
+    pop_frame();
+    let hReturn = ST.get () in
+    assume(is_poly_montgomery hReturn result)
 
 // This function is sometimes used with result and x the same, so we can't assume they are disjoint.
 val poly_sub_reduce:
